Rewrite comments

examples/add.s
@@ -1,5 +1,0 @@
-addi a0, a0, 1
-sb	 a0, 0(a1)
-jal a0, 0
-nop
-mret
