dorami/verification/F_universal_contract.v
@@ -2,6 +2,7 @@ From isla.dorami Require Import model.
 From isla.dorami Require Import later_lifting.
 
 (********************** Assumption Definitions Start ***********************)
+(** We try to make assumptions decidable(boolean). **)
 
 (* Some events don't have the operational semantics. *)
 Fixpoint NoEvent (t: isla_trace) : bool :=
@@ -50,11 +51,20 @@ Definition NoStuckEval (t: isla_trace) : Prop :=
 Scheme Equality for accessor.
 Scheme Equality for list.
 
+(* The deciable equality for the accessor list. *)
 Definition list_acc_eqb := list_beq accessor accessor_beq.
 Definition list_acc_eqb_eq a1 a2 : list_acc_eqb a1 a2 = true -> a1 = a2.
   refine (internal_list_dec_bl _ _ internal_accessor_dec_bl _ _).
 Defined.
 
+(* This definition list all the allowed registers in ReadReg which *)
+(* contains the PMP and MTVEC because we can read but cannot write it. *)
+(* This cumbersome definition is for the LegalRegAcc_R_destruct lemma. *)
+(* The problem stems from that the case match/destruct of string and list *)
+(* is very inconvenient. *)
+(* Here we only shows a small set of registers with different types as *)
+(* a proof of concept. *)
+(* TODO: With automation support, we support the full registers. *)
 Definition LegalRegAcc_R reg acc val : bool :=
   match val with
   | RVal_Bits bv =>
@@ -69,6 +79,8 @@ Definition LegalRegAcc_R reg acc val : bool :=
   | _ => false
   end.
 
+(* This definition list all the allowed registers in WriteReg that doesn't *)
+(* allow MTVEC or PMP compared with LegalRegAcc_R. *)
 Definition LegalRegAcc_W reg acc val : bool :=
   match val with
   | RVal_Bits bv =>
@@ -79,6 +91,32 @@ Definition LegalRegAcc_W reg acc val : bool :=
       (String.eqb reg "mcause" && (N.eqb (bvn_n bv) 64))
   | _ => false
   end.
+
+(* We requires that the top/head event satisfies the assumption *)
+(* LegalRegAcc_R. *)
+Definition LegalReadRegNow (t: isla_trace) : bool :=
+  match t with
+  | tnil => true
+  | tcons (ReadReg reg acc val _) t => LegalRegAcc_R reg acc val
+  | tcons _ t => true
+  | tcases ts => true
+  end.
+
+(* This property guaranteees that LegalRegAcc_R always holds during the *)
+(* evaluation of trace. *)
+Definition LegalReadReg (t: isla_trace) : Prop :=
+  t ≠ tnil -> forall t', rtc (fun t t' => ∃ label regs, trace_step t regs label t' ∧ label ≠ Some (LDone t')) t t' -> LegalReadRegNow t'.
+
+Definition LegalWriteRegNow (t: isla_trace) : bool :=
+  match t with
+  | tnil => true
+  | tcons (WriteReg reg acc val _) t => LegalRegAcc_W reg acc val
+  | tcons _ t => true
+  | tcases ts => true
+  end.
+
+Definition LegalWriteReg (t: isla_trace) : Prop :=
+  t ≠ tnil -> forall t', rtc (fun t t' => ∃ label regs, trace_step t regs label t' ∧ label ≠ Some (LDone t')) t t' -> LegalWriteRegNow t'.
 
 (* This is the complete the assumptions that F's code can have. *)
 (* This restriction makes sense because assume event can only come from *)
@@ -119,6 +157,8 @@ Definition assume_regs_map (mtvec: bv 64) : reg_map :=
   <[ "mtvec" := RegVal_Struct [("bits", RVal_Bits mtvec)] ]> $
   ∅.
 
+(* This definition list all the allowed registers in Assume. *)
+(* This is again a PoC that covers a small set of registers. *)
 Definition LegalAssumeEvent reg acc aval : bool :=
   match aval with
   | AVal_Var reg' acc' =>
@@ -148,6 +188,27 @@ Fixpoint LegalAssume (t: isla_trace) :=
   |tcases ts => forallb LegalAssume ts
   end.
 
+(* This definition lists all the registers in AssumeReg. *)
+Definition LegalRegAcc_A reg acc val : bool :=
+  match val with
+  | RVal_Bits bv =>
+      (String.eqb reg "rv_htif_tohost" && list_acc_eqb acc [] && (N.eqb (bvn_n bv) 64) && (Z.eqb (bvn_unsigned bv) 0x0000000040001000))
+      || (String.eqb reg "mseccfg" && list_acc_eqb acc [Field "bits"]
+       && (N.eqb (bvn_n bv) 64) && (Z.eqb (bvn_unsigned bv) 0x07))
+  | _ => false
+  end.
+
+Fixpoint LegalAssumeReg (t: isla_trace) : bool :=
+  match t with
+  | tnil => true
+  | tcons (AssumeReg reg acc val _)  t =>
+      LegalRegAcc_A reg acc val && LegalAssumeReg t
+  | tcons _ t => LegalAssumeReg t
+  | tcases ts => forallb LegalAssumeReg ts
+  end.
+
+(* This definition gives the restriction in memory access in *)
+(* Read/WriteMem events. *)
 Definition LegalMemAcc data addr len : bool :=
   (N.eqb (bvn_n addr) 64) && (N.eqb (bvn_n data) (8 * len))%N
   && (N.ltb 0 len)
@@ -181,21 +242,27 @@ Definition LegalWriteMemNow (t: isla_trace) : bool :=
 Definition LegalWriteMem (t: isla_trace) : Prop :=
   t ≠ tnil -> forall t', rtc (fun t t' => ∃ label regs, trace_step t regs label t' ∧ label ≠ Some (LDone t')) t t' -> LegalWriteMemNow t'.
 
+(* When the PC is misalinged or outside the authorized region, PC is *)
+(* updated to MTVEC right now. *)
 Definition illegal_PC `{!islaG Σ} `{!threadG} : iProp Σ :=
   ∀ i: bv 64, ("PC" ↦ᵣ RVal_Bits i ∗
   ⌜~ (bv_unsigned (bv_extract 0 2 i) = 0 ∧ (bv_unsigned F_code_addr) <= (bv_unsigned i) < (bv_unsigned F_code_end_addr))⌝)
        -∗ "PC" ↦ᵣ RVal_Bits F_mtvec.
 
+(* When cur_privilege is not in Machine, PC is updated to MTVEC right *)
+(* now and cur_privilege returns to Machine immediately. *)
+(* This is because there is no permission for other modes, which triggers *)
+(* the M-mode exception. *)
 Definition illegal_Priv `{!islaG Σ} `{!threadG} : iProp Σ :=
   ∀ i, "PC" ↦ᵣ i ∗ ("cur_privilege" ↦ᵣ: λ v, ⌜v ≠ RVal_Enum "Machine"⌝) -∗
   "PC" ↦ᵣ  RVal_Bits F_mtvec ∗ "cur_privilege" ↦ᵣ RVal_Enum "Machine".
 
 (*********************** Assumption Definitions End ************************)
 
-(********************* Properties of Assumption Start **********************)
+(********************* Properties of Assumptions Start *********************)
 
 (* The stronger induction principle for the proof that the property holds *)
-(* after the small-step opsem. *)
+(* after the small-step evaluations. *)
 Fixpoint isla_trace_custom_ind (P: isla_trace -> Prop) (Hnil: P tnil)
   (Hcon: ∀ e t, P t -> P (e :t: t))
   (Hcase: ∀ ts, Forall P ts -> P (tcases ts)) (i: isla_trace) {struct i} : P i
@@ -211,6 +278,8 @@ Fixpoint isla_trace_custom_ind (P: isla_trace -> Prop) (Hnil: P tnil)
                               (isla_trace_custom_ind P Hnil Hcon Hcase x) (forall_list t)
                     end) es)
   end.
+
+(* The NoEvent assumption holds during evaluation *)
 Lemma subst_trace_NoEvent v x t:
   NoEvent t -> NoEvent (subst_trace v x t).
 Proof.
@@ -238,6 +307,7 @@ Proof.
   by apply Is_true_true, Ht, elem_of_list_In.
 Qed.
 
+(* The NoEmptyCases assumption holds during evaluation *)
 Lemma subst_trace_NoEmptyCases v x t:
   NoEmptyCases t -> NoEmptyCases (subst_trace v x t).
 Proof.
@@ -275,39 +345,7 @@ Proof.
   by rewrite -elem_of_list_In.
 Qed.
 
-Lemma bv_extract_divisible {n} l (b : bv n) :
-  bv_unsigned (bv_extract 0 l b) = 0 -> ∃ quo, bv_unsigned b = 2 ^ Z.of_N l * quo.
-Proof.
-  rewrite bv_extract_unsigned /bv_wrap /bv_modulus.
-  replace (bv_unsigned b ≫ Z.of_N 0) with (bv_unsigned b) by done.
-  intro Hmod.
-  apply Z_div_exact_full_2 in Hmod; last lia.
-  by exists (bv_unsigned b `div` 2 ^ Z.of_N l).
-Qed.
-
-
-Definition LegalReadRegNow (t: isla_trace) : bool :=
-  match t with
-  | tnil => true
-  | tcons (ReadReg reg acc val _) t => LegalRegAcc_R reg acc val
-  | tcons _ t => true
-  | tcases ts => true
-  end.
-
-Definition LegalReadReg (t: isla_trace) : Prop :=
-  t ≠ tnil -> forall t', rtc (fun t t' => ∃ label regs, trace_step t regs label t' ∧ label ≠ Some (LDone t')) t t' -> LegalReadRegNow t'.
-
-Definition LegalWriteRegNow (t: isla_trace) : bool :=
-  match t with
-  | tnil => true
-  | tcons (WriteReg reg acc val _) t => LegalRegAcc_W reg acc val
-  | tcons _ t => true
-  | tcases ts => true
-  end.
-
-Definition LegalWriteReg (t: isla_trace) : Prop :=
-  t ≠ tnil -> forall t', rtc (fun t t' => ∃ label regs, trace_step t regs label t' ∧ label ≠ Some (LDone t')) t t' -> LegalWriteRegNow t'.
-
+(* Case match on the possible registers in ReadReg event. *)
 Lemma LegalRegAcc_R_destruct reg acc val :
   LegalRegAcc_R reg acc val->
     {bv | reg = "PC" ∧ acc = [] ∧ val = RVal_Bits bv ∧ (N.eqb (bvn_n bv) 64)} +
@@ -381,6 +419,7 @@ Definition bvn_to_bv'' b l v :
   by refine (match H with eq_refl => match H0 with eq_refl => _ end end).
 Defined.
 
+(* Case match on the possible registers in WriteReg event. *)
 Lemma LegalRegAcc_W_destruct reg acc val :
   LegalRegAcc_W reg acc val->
     {bv: bv 64 | reg = "PC" ∧ acc = [] ∧ val = RVal_Bits bv } +
@@ -450,15 +489,7 @@ Proof.
     by econstructor.
 Qed.
 
-Definition LegalRegAcc_A reg acc val : bool :=
-  match val with
-  | RVal_Bits bv =>
-      (String.eqb reg "rv_htif_tohost" && list_acc_eqb acc [] && (N.eqb (bvn_n bv) 64) && (Z.eqb (bvn_unsigned bv) 0x0000000040001000))
-      || (String.eqb reg "mseccfg" && list_acc_eqb acc [Field "bits"]
-       && (N.eqb (bvn_n bv) 64) && (Z.eqb (bvn_unsigned bv) 0x07))
-  | _ => false
-  end.
-
+(* Case matches for registers in AssumeReg. *)
 Lemma LegalRegAcc_A_destruct reg acc val :
   LegalRegAcc_A reg acc val->
     {bv | reg = "rv_htif_tohost" ∧ acc = [] ∧ val = RVal_Bits bv ∧ (bvn_n bv) = 64%N ∧ (bvn_unsigned bv) = 0x0000000040001000 } +
@@ -486,15 +517,6 @@ Proof.
       simplify_eq.
       by eauto 6.
 Qed.
-
-Fixpoint LegalAssumeReg (t: isla_trace) : bool :=
-  match t with
-  | tnil => true
-  | tcons (AssumeReg reg acc val _)  t =>
-      LegalRegAcc_A reg acc val && LegalAssumeReg t
-  | tcons _ t => LegalAssumeReg t
-  | tcases ts => forallb LegalAssumeReg ts
-  end.
 
 Lemma subst_trace_LegalAssumeReg v x t:
   LegalAssumeReg t -> LegalAssumeReg (subst_trace v x t).
@@ -693,6 +715,11 @@ Proof.
 Qed.
 (********************* Properties of Assumption End **********************)
 
+(* Because the instruction invariant can only be express by the weakestpre *)
+(* directly, we have to add PC permission and alignment and legal range *)
+(* conditions. *)
+(* The uni_csr and uni_gpr are machine_csr and machine_gpr with existential *)
+(* values because they can be changed by F. *)
 Definition F_with_PC (i: bv 64) `{!islaG Σ} `{!threadG} : iProp Σ :=
   "PC" ↦ᵣ RVal_Bits i ∗
   ⌜bv_unsigned (bv_extract 0 2 i) = 0⌝ ∗
@@ -1196,15 +1223,27 @@ Proof.
       by apply Hassume, elem_of_list_In.
 Qed.
 
-Definition universal_instrs `{!islaG Σ} `{!threadG} : iProp Σ :=
+(* This represents the instruction permission of F. *)
+Definition F_instrs `{!islaG Σ} `{!threadG} : iProp Σ :=
   ([∗ list] i ↦ _ ∈ replicate 1023 (), (∃ t, instr (0x80020000 + i * 4) (Some t) ∗ ⌜NoEmptyCases t ∧ NoEvent t ∧ NoStuckEval t ∧ LegalReadReg t ∧ LegalWriteReg t ∧ LegalReadMem t ∧ LegalWriteMem t ∧ LegalAssumeReg t ∧ LegalAssume t⌝)).
 
+(* The specification of the universal contract of F. *)
 Definition universal_spec `{!islaG Σ} `{!threadG} csr gpr mem : iProp Σ :=
   F F_mtvec F_pmpcfgs csr gpr mem ∗
   instr_pre (bv_unsigned SP_code_addr) (
      ∃ csr gpr mem, F F_mtvec SP_pmpcfgs csr gpr mem ∗
      True
 ).
+
+Lemma bv_extract_divisible {n} l (b : bv n) :
+  bv_unsigned (bv_extract 0 l b) = 0 -> ∃ quo, bv_unsigned b = 2 ^ Z.of_N l * quo.
+Proof.
+  rewrite bv_extract_unsigned /bv_wrap /bv_modulus.
+  replace (bv_unsigned b ≫ Z.of_N 0) with (bv_unsigned b) by done.
+  intro Hmod.
+  apply Z_div_exact_full_2 in Hmod; last lia.
+  by exists (bv_unsigned b `div` 2 ^ Z.of_N l).
+Qed.
 
 Theorem universal_contract `{!islaG Σ} `{!threadG} :
   ∀ (i: bv 64) csr gpr mem,
@@ -1213,7 +1252,7 @@ Theorem universal_contract `{!islaG Σ} `{!threadG} :
   length csr = 4%nat ->
   length gpr = 5%nat ->
   □ illegal_PC -∗
-  universal_instrs -∗
+  F_instrs -∗
   instr (bv_unsigned F_code_end_addr) (Some exit_firmware.a0.a0) -∗
   instr_body (bv_unsigned i) (universal_spec csr gpr mem).
 Proof.
